fmi/utp_hoare_ext.thy
@@ -1,0 +1,40 @@
+(******************************************************************************)
+(* Project: The Isabelle/UTP Proof System                                     *)
+(* File: utp_hoare_ext.thy                                                    *)
+(* Authors: Frank Zeyda and Simon Foster (University of York, UK)             *)
+(* Emails: frank.zeyda@york.ac.uk and simon.foster@york.ac.uk                 *)
+(******************************************************************************)
+
+section {* Hoare Logic Extensions *}
+
+theory utp_hoare_ext
+imports utp_hoare
+begin
+
+subsection {* Invariant Split Tactic *}
+
+text {* This tactic is slightly more efficient than @{method hoare_split}. *}
+
+named_theorems hoare_split_inv_laws "splitting laws for Hoare logic"
+
+lemmas seq_hoare_inv = seq_hoare_invariant
+
+lemma skip_hoare_aux:
+"\<lbrace>p \<and> q\<rbrace>II\<lbrace>p\<rbrace>\<^sub>u" by (rel_simp)+
+
+lemma cond_hoare_r':
+"\<lbrakk>\<lbrace>p \<and> b\<rbrace>S\<lbrace>q\<rbrace>\<^sub>u ; \<lbrace>p \<and> \<not>b\<rbrace>T\<lbrace>q\<rbrace>\<^sub>u\<rbrakk> \<Longrightarrow> \<lbrace>p\<rbrace>S \<triangleleft> b \<triangleright>\<^sub>r T\<lbrace>q\<rbrace>\<^sub>u"
+  by (rel_auto)
+
+declare hoare_r_conj [hoare_split_inv_laws]
+declare skip_hoare_r [hoare_split_inv_laws]
+declare skip_hoare_aux [hoare_split_inv_laws]
+declare assigns_hoare_r [hoare_split_inv_laws]
+declare seq_hoare_inv [hoare_split_inv_laws]
+declare cond_hoare_r' [hoare_split_inv_laws]
+declare while_hoare_r [hoare_split_inv_laws]
+declare while_invr_hoare_r [hoare_split_inv_laws]
+
+method hoare_split_inv uses add =
+  (rule hoare_split_inv_laws add; (hoare_split_inv add: add))?
+end
